Fix performances issues due to searching contradiction in the whole context (#34)
Closes: #33

The non-trivial closure rule now explicitly takes the relevant formulas.

---------

Co-authored-by: Julie Cailler <julie_cailler@hotmail.fr>

devtools/tests/rule_leaf.v
@@ -1,9 +1,12 @@
-
 Set Warnings "-native-compiler".
 From Tableaux Require Import All.
 
+Definition Axiom0 : EForm :=
+	EPred "a" [] 
+.
+
 Definition T : EForm :=
-	ENeg (EBot) 
+	EPred "a" [] 
 .
 
 Definition subst := translate_substitution [].
@@ -11,13 +14,11 @@ Definition subst := translate_substitution [].
 
 Definition T_Proof : ExtendedRuleTree.
 Proof.
-apply (mkUnaryNode ( AlphaNegNeg (Neg (Neg [[ EBot ]])) ) ).
-exact Leaf.
+exact (mkClosure [[ EPred "a" [] ]] [[ ENeg (EPred "a" []) ]]).
 Defined.
 
 Theorem hasTableau_T_Proof :
-	hasTableau InnerSkolemization [  Neg (translate_EForm T) ] subst.
+	hasTableau OuterSkolemization [  [[ Axiom0 ]] ;  Neg (translate_EForm T) ] subst.
 Proof.
 tableaux T_Proof.
 Qed.
-
