devtools/tests/rule_neg_neg.v
@@ -1,13 +1,12 @@
-
 Set Warnings "-native-compiler".
 From Tableaux Require Import All.
 
 Definition Axiom0 : EForm :=
-	EPred "a" [] 
+	ENeg (EPred "a" []) 
 .
 
 Definition T : EForm :=
-	EPred "a" [] 
+	ENeg (EPred "a" []) 
 .
 
 Definition subst := translate_substitution [].
@@ -15,12 +14,12 @@ Definition subst := translate_substitution [].
 
 Definition T_Proof : ExtendedRuleTree.
 Proof.
-exact Leaf.
+apply (mkUnaryNode ( AlphaNegNeg (Neg (Neg [[ EPred "a" [] ]])) ) ).
+exact (mkClosure [[ EPred "a" [] ]] [[ ENeg (EPred "a" []) ]]).
 Defined.
 
 Theorem hasTableau_T_Proof :
-	hasTableau InnerSkolemization [  [[ Axiom0 ]] ;  Neg (translate_EForm T) ] subst.
+	hasTableau OuterSkolemization [  [[ Axiom0 ]] ;  Neg (translate_EForm T) ] subst.
 Proof.
 tableaux T_Proof.
 Qed.
-
