devtools/tests/rule_all.v
@@ -1,4 +1,3 @@
-
 Set Warnings "-native-compiler".
 From Tableaux Require Import All.
 
@@ -14,12 +13,11 @@ Proof.
 apply (mkUnaryNode ( AlphaNegNeg (Neg (Neg [[ EAll "X3" (EAnd (EPred "p" [(EVar "X3")]) (ENeg (EPred "p" [(EVar "X3")]))) ]])) ) ).
 apply (mkUnaryNode ( GammaAll [[ EAll "X3" (EAnd (EPred "p" [(EVar "X3")]) (ENeg (EPred "p" [(EVar "X3")]))) ]] "X3_5" ) ).
 apply (mkUnaryNode ( AlphaAnd [[ EAnd (EPred "p" [(EVar "X3_5")]) (ENeg (EPred "p" [(EVar "X3_5")])) ]] ) ).
-exact Leaf.
+exact (mkClosure [[ EPred "p" [(EVar "X3_5")] ]] [[ ENeg (EPred "p" [(EVar "X3_5")]) ]]).
 Defined.
 
 Theorem hasTableau_T_Proof :
-	hasTableau InnerSkolemization [  Neg (translate_EForm T) ] subst.
+	hasTableau OuterSkolemization [  Neg (translate_EForm T) ] subst.
 Proof.
 tableaux T_Proof.
 Qed.
-
