devtools/tests/rule_neg_bot.v
@@ -1,9 +1,8 @@
-
 Set Warnings "-native-compiler".
 From Tableaux Require Import All.
 
 Definition T : EForm :=
-	EAnd (ETop) (ETop) 
+	ENeg (EBot) 
 .
 
 Definition subst := translate_substitution [].
@@ -11,18 +10,12 @@ Definition subst := translate_substitution [].
 
 Definition T_Proof : ExtendedRuleTree.
 Proof.
-apply (mkBinaryNode ( BetaNegAnd (Neg [[ EAnd (ETop) (ETop) ]]) ) ).
-{
-exact Leaf.
-}
-{
-exact Leaf.
-}
+apply (mkUnaryNode ( AlphaNegNeg (Neg (Neg [[ EBot ]])) ) ).
+exact mkTrivialClosure.
 Defined.
 
 Theorem hasTableau_T_Proof :
-	hasTableau InnerSkolemization [  Neg (translate_EForm T) ] subst.
+	hasTableau OuterSkolemization [  Neg (translate_EForm T) ] subst.
 Proof.
 tableaux T_Proof.
 Qed.
-
