devtools/tests/rule_neg_equ.v
@@ -1,0 +1,26 @@
+Set Warnings "-native-compiler".
+From Tableaux Require Import All.
+
+Definition T : EForm :=
+	EEqu (EPred "a" []) (EPred "a" []) 
+.
+
+Definition subst := translate_substitution [].
+
+
+Definition T_Proof : ExtendedRuleTree.
+Proof.
+apply (mkBinaryNode ( BetaNegEqu (Neg [[ EEqu (EPred "a" []) (EPred "a" []) ]]) ) ).
+{
+exact (mkClosure [[ EPred "a" [] ]] [[ ENeg (EPred "a" []) ]]).
+}
+{
+exact (mkClosure [[ EPred "a" [] ]] [[ ENeg (EPred "a" []) ]]).
+}
+Defined.
+
+Theorem hasTableau_T_Proof :
+	hasTableau OuterSkolemization [  Neg (translate_EForm T) ] subst.
+Proof.
+tableaux T_Proof.
+Qed.
