devtools/tests/rule_neg_ex.v
@@ -1,4 +1,3 @@
-
 Set Warnings "-native-compiler".
 From Tableaux Require Import All.
 
@@ -16,12 +15,11 @@ Definition subst := translate_substitution [("X4_6", (EFun "a" []))].
 Definition T_Proof : ExtendedRuleTree.
 Proof.
 apply (mkUnaryNode ( GammaNegEx (Neg [[ EEx "X4" (EPred "p" [(EVar "X4")]) ]]) "X4_6" ) ).
-exact Leaf.
+exact (mkClosure [[ ENeg (EPred "p" [(EVar "X4_6")]) ]] [[ EPred "p" [(EFun "a" [])] ]]).
 Defined.
 
 Theorem hasTableau_T_Proof :
-	hasTableau InnerSkolemization [  [[ Axiom0 ]] ;  Neg (translate_EForm T) ] subst.
+	hasTableau OuterSkolemization [  [[ Axiom0 ]] ;  Neg (translate_EForm T) ] subst.
 Proof.
 tableaux T_Proof.
 Qed.
-
